tests/csample2/test.ml
@@ -13,11 +13,11 @@ let () =
   match CPolIRs.scheduler cpol_orig with
   | Okk cpol_opt -> 
       cpol_printer "./opt.cpol" cpol_opt;
-      let (res, ok) = CPolOpt.Validator.validate cpol_orig cpol_opt in
+      let (res, ok) = CPolOpt.validate cpol_orig cpol_opt in
       (* printf "%b\n" res; *)
       (if ok && res then printf "\027[32mSUCCEED\027[0m: (orig -> opt).\n"
       else printf "\027[31mFAIL\027[0m: (orig -> opt).\n");
-      let (res, ok) = CPolOpt.Validator.validate cpol_opt cpol_orig  in
+      let (res, ok) = CPolOpt.validate cpol_opt cpol_orig  in
       (* printf "%b\n" res; *)
       (if ok && res then printf "\027[32mSUCCEED\027[0m: (opt -> orig).\n"
       else printf "\027[31mFAIL\027[0m: (opt -> orig).\n");
