driver/TPolValidator.v
@@ -1,9 +1,8 @@
 Require Import TPolIRs.
-Require Import Validator.
 Require Import ImpureAlarmConfig.
 Require Import Vpl.Impure.
-(** The final polyhedral optimizer *)
-
 Require Import PolOpt.
+
 Module TValidatorOpt := PolOpt TPolIRs.
-Module TVal := TValidatorOpt.Validator.
+
+Definition validate := TValidatorOpt.ValidatorCore.validate.
