syntax/SPolIRs.v
@@ -78,7 +78,11 @@ Module SPolIRs <: POLIRS with Module Instr := SInstr.
         end
     | None => Err "Transform pol to openscop failed"
     end.
+  Definition affine_scheduler := scheduler.
 
-  Definition to_phase_openscop (cpol: PolyLang.t) : option OpenScop :=
+  Definition export_for_phase_scheduler (cpol: PolyLang.t) : option OpenScop :=
     to_openscop_source cpol.
+  Definition export_for_pluto_phase_pipeline := export_for_phase_scheduler.
+  Definition to_phase_openscop := export_for_phase_scheduler.
+  Definition run_pluto_phase_pipeline := phase_scop_scheduler.
 End SPolIRs.
